theories/stacked_borrows/examples/opt1.v
@@ -148,11 +148,12 @@ Proof.
 Qed.
 
 
-
+(** A variant of this optimization (actually the one from the original formalization)
+  which uses deferred UB. *)
 Definition ex1_opt' : ectx :=
   λ: "i",
     let: "x" := new_place (&mut int) "i" in
-    retag_place "x" (RefPtr Mutable) int Default "c";;
+    retag_place "x" (RefPtr Mutable) int Default #[ScCallId 0];;
     Call #[ScFnPtr "f"] #[] ;;
     *{int} "x" <- #[42] ;;
     (* using a read here: requires to use LLVM semantics for reads *)
@@ -164,4 +165,67 @@ Definition ex1_opt' : ectx :=
 Lemma sim_opt1' `{sborG Σ} π :
   ⊢ sim_ectx rrel π ex1_opt' ex1_unopt rrel.
 Proof.
-Abort.
+  iIntros (r_t r_s) "Hrel".
+  sim_pures.
+  sim_apply (Alloc _) (Alloc _) sim_alloc_local "". iIntros (t l) "Htag Ht Hs".
+  iApply sim_expr_base. sim_pures.
+
+  source_bind (Write _ _).
+  destruct r_s as [v_s | ]; first last.
+  { iApply source_red_irred_unless; first done. by iIntros. }
+  (* gain knowledge about the length *)
+  iApply source_red_irred_unless; first done. iIntros (Hsize).
+  iApply (source_write_local with "Htag Hs"); [by rewrite repeat_length | done | ].
+  iIntros "Hs Htag". source_finish.
+  iPoseProof (rrel_value_source with "Hrel") as (v_t) "(-> & #Hv)".
+  iPoseProof (value_rel_length with "Hv") as "%Hlen".
+  target_apply (Write _ _) (target_write_local with "Htag Ht") "Ht Htag"; [ by rewrite repeat_length | lia| ].
+  sim_pures.
+
+  target_apply (Copy _) (target_copy_local with "Htag Ht") "Ht Htag"; first lia.
+  source_apply (Copy _) (source_copy_local with "Htag Hs") "Hs Htag"; first lia.
+
+  (* do the retag *)
+  sim_bind (Retag _ _ _ _ _) (Retag _ _ _ _ _).
+  iApply sim_irred_unless; first done.
+  iIntros ((_ & ot & i & -> & _)).
+  iPoseProof (value_rel_singleton_source with "Hv") as (sc_t) "[-> Hscrel]".
+  iPoseProof (sc_rel_ptr_source with "Hscrel") as "[-> Htagged]".
+  iApply (sim_retag_default with "Hscrel"); [cbn; lia| done | ].
+  iIntros (t_i v_t v_s Hlen_t Hlen_s) "_ Htag_i Hi_t Hi_s _".
+  iApply sim_expr_base.
+  target_apply (Write _ _) (target_write_local with "Htag Ht") "Ht Htag"; [done | done | ].
+  source_apply (Write _ _) (source_write_local with "Htag Hs") "Hs Htag"; [done | done | ].
+  sim_pures.
+
+  sim_apply (Call _ _) (Call _ _) (sim_call _ _ (ValR []) (ValR [])) ""; first by iApply value_rel_empty.
+  iIntros (r_t r_s) "_". sim_pures.
+
+  target_apply (Copy _) (target_copy_local with "Htag Ht") "Ht Htag"; first done.
+  source_apply (Copy _) (source_copy_local with "Htag Hs") "Hs Htag"; first done.
+  sim_pures.
+
+  (* we need to do the writes symmetrically: we cannot know if the tag is still on top *)
+  sim_apply (Write _ _) (Write _ _) (sim_write_unique_unprotected with "Htag_i Hi_t Hi_s") "Htag_i Hi_t Hi_s".
+  sim_pures.
+
+  (* deferred read in the target *)
+  target_apply (Copy (Place _ _ _)) (target_copy_local with "Htag Ht") "Ht Htag"; first done.
+  target_pures. target_bind (Copy _).
+  iApply (target_copy_deferred with "Htag_i Hi_t"); first done. iIntros (v_t') "Hdeferred Hi_t Htag_i". target_finish.
+  sim_pures.
+
+  sim_apply (Call _ _) (Call _ _) (sim_call _ _ (ValR []) (ValR [])) ""; first by iApply value_rel_empty.
+  iIntros (r_t' r_s') "_". sim_pures.
+
+  (* resolve the deferred read in the source *)
+  source_apply (Copy (Place _ _ _)) (source_copy_local with "Htag Hs") "Hs Htag"; first done.
+  source_pures. source_bind (Copy _).
+  iApply (source_copy_resolve_deferred with "Htag_i Hi_s Hdeferred"); first done. 
+  { iApply big_sepL2_singleton. done. } 
+  iIntros (v_s') "Hv' Hi_s Htag_i". source_finish.
+  sim_pures.
+
+  sim_apply (Free _) (Free _) (sim_free_local with "Htag Ht Hs") "". sim_pures.
+  sim_val. iModIntro. done.
+Qed.
